wip

template-coq/theories/kernel/wGraph.v
@@ -3,6 +3,8 @@ Require Import Peano_dec Nat Bool List Structures.Equalities Lia
 Require Import ssrbool ssrfun.
  From Template Require Import utils monad_utils.
 
+ Axiom myadmit : forall {A}, A.
+
 Inductive on_Some {A} (P : A -> Prop) : option A -> Prop :=
 | on_some : forall x, P x -> on_Some P (Some x).
 
@@ -88,6 +90,10 @@ Module Nbar.
     | Some _, None => False
     | None, _ => True
     end.
+
+  Arguments max _ _ : simpl nomatch.
+  Arguments add _ _ : simpl nomatch.
+  Arguments le _ _ : simpl nomatch.
 
   Infix "+" := add : nbar_scope.
   Infix "<=" := le : nbar_scope.
@@ -263,31 +269,31 @@ Module WeightedGraph (V : UsualOrderedType).
     Definition lt_compat : Proper (Logic.eq ==> Logic.eq ==> iff) lt.
       intros x x' H1 y y' H2. now subst.
     Qed.
-   Definition compare : t -> t -> comparison
-     := fun '(x, n, y) '(x', n', y') => match V.compare x x' with
-                                     | Lt => Lt
-                                     | Gt => Gt
-                                     | Eq => match PeanoNat.Nat.compare n n' with
-                                            | Lt => Lt
-                                            | Gt => Gt
-                                            | Eq => V.compare y y'
-                                            end
-                                     end.
-   Definition compare_spec :
-     forall x y : t, CompareSpec (x = y) (lt x y) (lt y x) (compare x y).
-     intros [[x1 n1] y1] [[x2 n2] y2]; cbn.
-     pose proof (V.compare_spec x1 x2) as H1.
-     destruct (V.compare x1 x2); cbn in *; inversion_clear H1.
-     2-3: constructor; intuition.
-     subst. pose proof (PeanoNat.Nat.compare_spec n1 n2) as H2.
-     destruct (n1 ?= n2); cbn in *; inversion_clear H2.
-     2-3: constructor; intuition.
-     subst. pose proof (V.compare_spec y1 y2) as H3.
-     destruct (V.compare y1 y2); cbn in *; inversion_clear H3;
-       constructor; subst; intuition.
-   Defined.
-     
-   Definition eq_dec : forall x y : t, {x = y} + {x <> y}.
+    Definition compare : t -> t -> comparison
+      := fun '(x, n, y) '(x', n', y') => match V.compare x x' with
+                                      | Lt => Lt
+                                      | Gt => Gt
+                                      | Eq => match PeanoNat.Nat.compare n n' with
+                                             | Lt => Lt
+                                             | Gt => Gt
+                                             | Eq => V.compare y y'
+                                             end
+                                      end.
+    Definition compare_spec :
+      forall x y : t, CompareSpec (x = y) (lt x y) (lt y x) (compare x y).
+      intros [[x1 n1] y1] [[x2 n2] y2]; cbn.
+      pose proof (V.compare_spec x1 x2) as H1.
+      destruct (V.compare x1 x2); cbn in *; inversion_clear H1.
+      2-3: constructor; intuition.
+      subst. pose proof (PeanoNat.Nat.compare_spec n1 n2) as H2.
+      destruct (n1 ?= n2); cbn in *; inversion_clear H2.
+      2-3: constructor; intuition.
+      subst. pose proof (V.compare_spec y1 y2) as H3.
+      destruct (V.compare y1 y2); cbn in *; inversion_clear H3;
+        constructor; subst; intuition.
+    Defined.
+    
+    Definition eq_dec : forall x y : t, {x = y} + {x <> y}.
       unfold eq. decide equality. apply V.eq_dec.
       decide equality. apply PeanoNat.Nat.eq_dec. apply V.eq_dec.
     Defined.
@@ -317,14 +323,6 @@ Module WeightedGraph (V : UsualOrderedType).
 
   Section graph.
     Context (G : t).
-
-    Definition invariants :=
-      (* E ⊆ V × V *)
-      (forall e, EdgeSet.In e (E G) -> VSet.In e..s (V G) /\ VSet.In e..t (V G)).
-      (* (* s ∈ V *) *)
-      (* /\  VSet.In (s G) (V G) *)
-      (* (* s is a source *) *)
-      (* /\ (forall x, VSet.In x (V G) -> Rs (s G) x). *)
 
     Definition add_node x : t :=
       (VSet.add x (V G), (E G), (s G)).
@@ -367,7 +365,37 @@ Module WeightedGraph (V : UsualOrderedType).
     Global Instance Paths_refl : CRelationClasses.Reflexive Paths := paths_refl.
     Global Instance Paths_trans : CRelationClasses.Transitive Paths := @concat.
 
+
+    Definition invariants :=
+      (* E ⊆ V × V *)
+      (forall e, EdgeSet.In e (E G) -> VSet.In e..s (V G) /\ VSet.In e..t (V G))
+      (* s ∈ V *)
+      /\  VSet.In (s G) (V G)
+      (* s is a source *)
+      /\ (forall x, VSet.In x (V G) -> ∥ Paths (s G) x ∥).
+
+    Context (HI : invariants).
+
+
     Definition PosPaths x y := exists p : Paths x y, weight p > 0.
+
+    Definition acyclic_no_loop := forall x (p : Paths x x), weight p = 0.
+
+    Definition acyclic_no_loop' := forall x, ~ (PosPaths x x).
+
+    Fact acyclic_no_loop_loop' : acyclic_no_loop <-> acyclic_no_loop'.
+    Proof.
+      unfold acyclic_no_loop, acyclic_no_loop', PosPaths.
+      split.
+      - intros H x [p HH]. specialize (H x p); lia.
+      - intros H x p.
+        destruct (PeanoNat.Nat.eq_0_gt_0_cases (weight p));
+          firstorder.
+    Qed.
+
+
+
+
 
     Definition DisjointAdd x s s' := VSetProp.Add x s s' /\ ~ VSet.In x s.
 
@@ -393,6 +421,12 @@ Module WeightedGraph (V : UsualOrderedType).
       | spaths_step _ _ x y z _ e p => e..1 + sweight p
       end.
 
+    Lemma sweight_weight {s x y} (p : SimplePaths s x y)
+      : sweight p = weight (to_paths p).
+    Proof.
+      induction p; cbn; lia.
+    Qed.
+
     Fixpoint is_simple {x y} (p : Paths x y) :=
       match p with
       | paths_refl x => true
@@ -416,42 +450,77 @@ Module WeightedGraph (V : UsualOrderedType).
       rewrite Hp in Heq_p. cbn in Heq_p; now apply andb_prop, proj2 in Heq_p.
     Defined.
 
-    Lemma DisjointAdd_add {s s' x y} (H : DisjointAdd x s s') (H' : x <> y)
-      : DisjointAdd x (VSet.add y s) (VSet.add y s').
+
+    (* Lemma DisjointAdd_add {s s' x y} (H : DisjointAdd x s s') (H' : x <> y) *)
+    (*   : DisjointAdd x (VSet.add y s) (VSet.add y s'). *)
+    (* Proof. *)
+    (*   repeat split. 2: intros [H0|H0]. *)
+    (*  - intro H0. apply VSet.add_spec in H0. *)
+    (*    destruct H0 as [H0|H0]. *)
+    (*    right; subst; apply VSet.add_spec; left; reflexivity. *)
+    (*    apply H in H0. destruct H0 as [H0|H0]; [left; assumption |right]. *)
+    (*    apply VSet.add_spec; right; assumption. *)
+    (*  - subst. apply VSet.add_spec; right. apply H; left; reflexivity. *)
+    (*  - apply VSet.add_spec in H0; apply VSet.add_spec; destruct H0 as [H0|H0]. *)
+    (*    left; assumption. right. apply H. right; assumption. *)
+    (*  - intro H0. apply VSet.add_spec in H0; destruct H0 as [H0|H0]. *)
+    (*    contradiction. now apply H. *)
+    (* Qed. *)
+
+    Lemma DisjointAdd_add1 {s0 s1 s2 x y}
+          (H1 : DisjointAdd x s0 s1) (H2 : DisjointAdd y s1 s2)
+      : DisjointAdd x (VSet.add y s0) s2.
     Proof.
-      repeat split. 2: intros [H0|H0].
-     - intro H0. apply VSet.add_spec in H0.
-       destruct H0 as [H0|H0].
-       right; subst; apply VSet.add_spec; left; reflexivity.
-       apply H in H0. destruct H0 as [H0|H0]; [left; assumption |right].
-       apply VSet.add_spec; right; assumption.
-     - subst. apply VSet.add_spec; right. apply H; left; reflexivity.
-     - apply VSet.add_spec in H0; apply VSet.add_spec; destruct H0 as [H0|H0].
-       left; assumption. right. apply H. right; assumption.
-     - intro H0. apply VSet.add_spec in H0; destruct H0 as [H0|H0].
-       contradiction. now apply H.
+      split.
+      intro z; split; intro Hz. 2: destruct Hz as [Hz|Hz].
+      - apply H2 in Hz. destruct Hz as [Hz|Hz]; [right|].
+        now apply VSetFact.add_1.
+        apply H1 in Hz. destruct Hz as [Hz|Hz]; [left; assumption|right].
+        now apply VSetFact.add_2.
+      - apply H2. right; apply H1. now left.
+      - apply H2. apply VSet.add_spec in Hz.
+        destruct Hz as [Hz|Hz]; [now left|right].
+        apply H1. now right.
+      - intro Hx. apply VSet.add_spec in Hx.
+        destruct Hx as [Hx|Hx].
+        subst. apply H2. apply H1. now left.
+        now apply H1.
+    Qed.
+
+    Lemma DisjointAdd_add2 {s x} (H : ~ VSet.In x s)
+      : DisjointAdd x s (VSet.add x s).
+    Proof.
+      split. apply VSetProp.Add_add.
+      assumption.
+    Qed.
+
+    Lemma DisjointAdd_add3  {s0 s1 s2 x y}
+          (H1 : DisjointAdd x s0 s1) (H2 : DisjointAdd y s1 s2)
+      : DisjointAdd y s0 (VSet.add y s0).
+    Proof.
+      apply DisjointAdd_add2. intro H.
+      unfold DisjointAdd in *.
+      apply H2. apply H1. now right.
     Qed.
 
 
-    Program Fixpoint add_end {s x y} (p : SimplePaths s x y)
-      : forall {z} (e : Edges y z) (Hy : ~ VSet.In y s), SimplePaths (VSet.add y s) x z
+    Fixpoint add_end {s x y} (p : SimplePaths s x y)
+      : forall {z} (e : Edges y z) {s'} (Hs : DisjointAdd y s s'), SimplePaths s' x z
       := match p with
-         | spaths_refl s x => fun z e Hy => spaths_step _ e (spaths_refl _ _)
-         | spaths_step s s' _ _ _ H e p
-           => fun z e' Hy => spaths_step _ e (add_end p e' _)
+         | spaths_refl s x => fun z e s' Hs => spaths_step Hs e (spaths_refl _ _)
+         | spaths_step s0 s x x0 y H e p
+           => fun z e' s' Hs => spaths_step (DisjointAdd_add1 H Hs) e
+                                        (add_end p e' (DisjointAdd_add3 H Hs))
          end.
-    Next Obligation.
-      cbn. split. apply VSetProp.Add_add. assumption.
-    Defined.
-    Next Obligation.
-      apply DisjointAdd_add. assumption.
-      intro HH; apply Hy.  apply H. left; assumption.
-    Defined.
-    Next Obligation.
-      intro HH. apply Hy. apply H. right; assumption.
-    Defined.
 
-    Axiom myadmit : forall {A}, A.
+    Lemma weight_add_end {s x y} (p : SimplePaths s x y) {z e s'} Hs
+      : sweight (@add_end s x y p z e s' Hs) = sweight p + e..1.
+    Proof.
+      revert z e s' Hs. induction p.
+      - intros; cbn; lia.
+      - intros; cbn. rewrite IHp; lia.
+    Qed.
+
 
     Lemma DisjointAdd_remove {s s' x y} (H : DisjointAdd x s s') (H' : x <> y)
       : DisjointAdd x (VSet.remove y s) (VSet.remove y s').
@@ -471,34 +540,150 @@ Module WeightedGraph (V : UsualOrderedType).
        apply H; assumption.
     Qed.
 
+   (* Fixpoint split {s x y} (p : SimplePaths s x y) *)
+   (*   : SimplePaths (VSet.remove y s) x y * ∑ s', SimplePaths s' y y := *)
+   (*    match p with *)
+   (*    | spaths_refl s x => (spaths_refl _ x, (VSet.empty; spaths_refl _ x)) *)
+   (*    | spaths_step s s' x0 y0 z0 H e p0 *)
+   (*      => match V.eq_dec x0 z0 with *)
+   (*        | left pp => (eq_rect _ (SimplePaths _ _) (spaths_refl _ _) _ pp, *)
+   (*                     (s'; eq_rect _ (fun x => SimplePaths _ x _) *)
+   (*                                  (spaths_step H e p0) _ pp)) *)
+   (*        | right pp => (spaths_step (DisjointAdd_remove H pp) e (split p0).1, *)
+   (*                      (split p0).2) *)
+   (*        end *)
+   (*    end. *)
 
+    Definition SimplePaths_sub {s s' x y}
+      : VSet.Subset s s' -> SimplePaths s x y -> SimplePaths s' x y.
+    Proof.
+      intros Hs p; revert s' Hs; induction p.
+      - reflexivity.
+      - intros s'0 Hs. unshelve econstructor.
+        exact (VSet.remove x s'0).
+        3: eassumption. 2: eapply IHp.
+        + split. apply VSetProp.Add_remove.
+          apply Hs, d; intuition.
+          now apply VSetProp.FM.remove_1.
+        + intros u Hu. apply VSetFact.remove_2.
+          intro X. apply d. subst; assumption.
+          apply Hs, d; intuition.
+    Defined.
+
+    Definition weight_SimplePaths_sub {s s' x y} Hs p
+      : sweight (@SimplePaths_sub s s' x y Hs p) = sweight p.
+    Proof.
+      revert s' Hs; induction p; simpl. reflexivity.
+      intros s'0 Hs. now rewrite IHp.
+    Qed.
+
+    Lemma DisjointAdd_Subset {x s s'}
+      : DisjointAdd x s s' -> VSet.Subset s s'.
+    Proof.
+      intros [H _] z Hz. apply H; intuition.
+    Qed.
 
    Fixpoint split {s x y} (p : SimplePaths s x y)
-     : SimplePaths (VSet.remove y s) x y * ∑ s', SimplePaths s' y y :=
+     : SimplePaths (VSet.remove y s) x y * SimplePaths s y y :=
       match p with
-      | spaths_refl s x => (spaths_refl _ x, (VSet.empty; spaths_refl _ x))
+      | spaths_refl s x => (spaths_refl _ x, spaths_refl _ x)
       | spaths_step s s' x0 y0 z0 H e p0
         => match V.eq_dec x0 z0 with
           | left pp => (eq_rect _ (SimplePaths _ _) (spaths_refl _ _) _ pp,
-                       (s'; eq_rect _ (fun x => SimplePaths _ x _)
-                                    (spaths_step H e p0) _ pp))
+                       eq_rect _ (fun x => SimplePaths _ x _) (spaths_step H e p0) _ pp)
           | right pp => (spaths_step (DisjointAdd_remove H pp) e (split p0).1,
-                        (split p0).2)
+                        SimplePaths_sub (DisjointAdd_Subset H) (split p0).2)
           end
       end.
+
+    Lemma weight_split {s x y} (p : SimplePaths s x y)
+      : sweight (split p).1 + sweight (split p).2 = sweight p.
+    Proof.
+      induction p.
+      - reflexivity.
+      - simpl. destruct (V.eq_dec x z).
+        + destruct e0; cbn. reflexivity.
+        + cbn. rewrite weight_SimplePaths_sub; lia.
+    Qed.
+
+    Lemma DisjointAdd_remove1 {s x} (H : VSet.In x s)
+      : DisjointAdd x (VSet.remove x s) s.
+    Proof.
+      split.
+      - intro z; split; intro Hz. 2: destruct Hz as [Hz|Hz].
+        + destruct (V.eq_dec x z). now left.
+          right. now apply VSetFact.remove_2.
+        + now subst.
+        + eapply VSetFact.remove_3; eassumption.
+      - now apply VSetFact.remove_1.
+    Qed.
+
+    Lemma Add_In {s x} (H : VSet.In x s)
+      : VSetProp.Add x s s.
+    Proof.
+      split. intuition.
+      intros []; try subst; assumption.
+    Qed.
+
+    Lemma Add_Add {s s' x} (H : VSetProp.Add x s s')
+      : VSetProp.Add x s' s'.
+    Proof.
+      apply Add_In, H. left; reflexivity.
+    Qed.
+
+
+    Lemma simplify_aux1 {s0 s1 s2} (H : VSet.Equal (VSet.union s0 s1) s2)
+      : VSet.Subset s0 s2.
+    Proof.
+      intros x Hx. apply H.
+      now apply VSetFact.union_2.
+    Qed.
  
+    Lemma simplify_aux2 {s0 x} (Hx : VSet.mem x s0 = true)
+          {s1 s2}
+          (Hs : VSet.Equal (VSet.union s0 (VSet.add x s1)) s2)
+      : VSet.Equal (VSet.union s0 s1) s2.
+    Proof.
+      apply VSet.mem_spec in Hx.
+      etransitivity; [|eassumption].
+      intro y; split; intro Hy; apply VSet.union_spec;
+        apply VSet.union_spec in Hy; destruct Hy as [Hy|Hy].
+      left; assumption.
+      right; now apply VSetFact.add_2.
+      left; assumption.
+      apply VSet.add_spec in Hy; destruct Hy as [Hy|Hy].
+      left; subst; assumption.
+      right; assumption.
+    Qed.
+
+    Lemma simplify_aux3 {s0 s1 s2 x}
+          (Hs : VSet.Equal (VSet.union s0 (VSet.add x s1)) s2)
+      : VSet.Equal (VSet.union (VSet.add x s0) s1) s2.
+    Proof.
+      etransitivity; [|eassumption].
+      etransitivity. eapply VSetProp.union_add.
+      symmetry. etransitivity. apply VSetProp.union_sym.
+      etransitivity. eapply VSetProp.union_add.
+      apply VSetFact.add_m. reflexivity.
+      apply VSetProp.union_sym.
+    Qed.
+
     Fixpoint simplify {s x y} (q : Paths y x)
-      : SimplePaths s x y -> ∑ x' s', SimplePaths s' x' x' :=
+      : forall (p : SimplePaths s x y) {s'},
+        VSet.Equal (VSet.union s (nodes q)) s' -> ∑ x', SimplePaths s' x' x' :=
       match q with
-      | paths_refl x => fun p => (x; s; p)
+      | paths_refl x => fun p s' Hs => (x; SimplePaths_sub (simplify_aux1 Hs) p)
       | paths_step y y' _ e q =>
-        fun p => match VSet.mem y s as X return VSet.mem y s = X -> _ with
+        fun p s' Hs => match VSet.mem y s as X return VSet.mem y s = X -> _ with
               | true => fun XX => let '(p1, p2) := split p in
-                       if 0 <? sweight (p2..2) then (_; p2)
-                       else simplify q
-                                  (add_end p1 e (VSetProp.FM.remove_1 eq_refl))
-              | false => fun XX => simplify q (add_end p e
-                                  ((VSetFact.not_mem_iff _ _).2 XX))
+                       if 0 <? sweight p2
+                       then (y; SimplePaths_sub (simplify_aux1 Hs) p2)
+                       else (simplify q (add_end p1 e
+                                          (DisjointAdd_remove1 (VSetFact.mem_2 XX)))
+                                      (simplify_aux2 XX Hs))
+              | false => fun XX => (simplify q (add_end p e
+                            (DisjointAdd_add2 ((VSetFact.not_mem_iff _ _).2 XX)))
+                                         (simplify_aux3 Hs))
               end eq_refl
       end.
 
@@ -522,37 +707,46 @@ Module WeightedGraph (V : UsualOrderedType).
     (*   now apply VSetFact.not_mem_iff. *)
     (* Defined. *)
 
-    Lemma weight_split {s x y} (p : SimplePaths s x y)
-      : sweight (split p).1 + sweight (split p).2..2 = sweight p.
-    Proof.
-      induction p.
-      - reflexivity.
-      - simpl. destruct (V.eq_dec x z).
-        + destruct e0; cbn. reflexivity.
-        + cbn. lia.
-    Qed.
+    (* Lemma weight_simplify (HG : acyclic_no_loop) {s x y} q (p : SimplePaths s x y) *)
+    (*   : 0 < weight q \/ 0 < sweight p -> 0 < sweight (simplify q p)..2..2. *)
+    (* Proof. *)
+    (*   revert s p; induction q. *)
+    (*   - cbn. intuition. *)
+    (*   - intros s p H; cbn in H. simpl. *)
+    (*     set (F := proj2 (VSetFact.not_mem_iff s x)); clearbody F. *)
+    (*     destruct (VSet.mem x s). *)
+    (*     + case_eq (split p); intros p1 p2 Hp. *)
+    (*       case_eq (0 <? sweight p2..2); intro eq. *)
+    (*       cbn. apply PeanoNat.Nat.leb_le in eq. lia. *)
+    (*       eapply IHq. rewrite weight_add_end. *)
+    (*       pose proof (weight_split p) as X; rewrite Hp in X. *)
+    (*       destruct p2 as  [s' p2]; simpl in *. *)
+    (*       pose proof (sweight_weight p2) as HH. *)
+    (*       rewrite HG in HH. lia. *)
+    (*     + eapply IHq. rewrite weight_add_end. *)
+    (*       lia. *)
+    (* Qed. *)
 
     Lemma weight_simplify {s x y} q (p : SimplePaths s x y)
-      : 0 < weight q \/ 0 < sweight p -> 0 < sweight (simplify q p)..2..2.
+      : forall {s'} Hs, 0 < weight q \/ 0 < sweight p
+        -> 0 < sweight (simplify q p (s':=s') Hs)..2.
     Proof.
-      revert p; induction q.
-      - cbn. intuition.
-      - intros p H; cbn in H. simpl.
-        set (F := proj2 (VSetFact.not_mem_iff s x)); clearbody F.
+      revert s p; induction q.
+      - cbn; intros. intuition. now rewrite weight_SimplePaths_sub.
+      - intros s p s' Hs H; cbn in H. simpl.
+        set (F0 := proj2 (VSetFact.not_mem_iff s x)); clearbody F0.
+        set (F1 := @VSetFact.mem_2 s x); clearbody F1.
+        set (F2 := @simplify_aux2 s x); clearbody F2.
         destruct (VSet.mem x s).
         + case_eq (split p); intros p1 p2 Hp.
-          case_eq (0 <? sweight p2..2); intro eq.
-          cbn. apply PeanoNat.Nat.leb_le in eq. lia.
-          admit.
-        + eapply (IHq (add_end p e (F (erefl false)))).
-          eapply IHq.
-        destruct X.
-
-
-        clearbody eq; change (VSet.mem x s = X) in eq.
-        case X. clearbody X.
-        pose proof (Sumbool.sumbool_of_bool X) as XX; destruct XX as [XX|XX].
-        rewrite XX.
+          case_eq (0 <? sweight p2); intro eq.
+          cbn. apply PeanoNat.Nat.leb_le in eq.
+          rewrite weight_SimplePaths_sub; lia.
+          eapply IHq. rewrite weight_add_end.
+          pose proof (weight_split p) as X; rewrite Hp in X; cbn in X.
+          apply PeanoNat.Nat.ltb_ge in eq. lia.
+        + eapply IHq. rewrite weight_add_end. lia.
+    Qed.
 
 
 
@@ -565,19 +759,22 @@ Module WeightedGraph (V : UsualOrderedType).
     (* lsp = longest simple path *)
     (* l is the list of authorized intermediate nodes *)
     (* lsp0 (a::l) x y = max (lsp0 l x y) (lsp0 l x a + lsp0 l a y) *)
-    Program Fixpoint lsp0 (s : VSet.t) (x z : V.t) {measure (VSet.cardinal s)}
-      : Nbar.t :=
+
+    Fixpoint lsp00 fuel (s : VSet.t) (x z : V.t) : Nbar.t :=
       let base := if V.eq_dec x z then Some 0 else None in
-      match VSet.mem x s with
-      | true =>
-        let ds := List.map (fun '(n, y) => Some n + lsp0 (VSet.remove x s) y z)%nbar
-                           (succs x) in
-        List.fold_left Nbar.max ds base
-      | false => base end.
-    Next Obligation.
-      symmetry in Heq_anonymous0; apply VSet.mem_spec in Heq_anonymous0.
-      apply VSetProp.remove_cardinal_1 in Heq_anonymous0. lia.
-    Defined.
+      match fuel with
+      | 0 => base
+      | S fuel => 
+        match VSet.mem x s with
+        | true =>
+          let ds := List.map
+                      (fun '(n, y) => Some n + lsp00 fuel (VSet.remove x s) y z)%nbar
+                      (succs x) in
+          List.fold_left Nbar.max ds base
+        | false => base end
+      end.
+
+    Definition lsp0 s := lsp00 (VSet.cardinal s) s.
 
     Lemma lsp0_eq s x z : lsp0 s x z =
       let base := if V.eq_dec x z then Some 0 else None in
@@ -588,15 +785,51 @@ Module WeightedGraph (V : UsualOrderedType).
         List.fold_left Nbar.max ds base
       | false => base end.
     Proof.
-    Admitted.
+      unfold lsp0. set (fuel := VSet.cardinal s).
+      cut (VSet.cardinal s = fuel); [|reflexivity].
+      clearbody fuel. revert s x. induction fuel.
+      - intros s x H.
+        apply VSetProp.cardinal_inv_1 in H.
+        specialize (H x). apply VSetProp.FM.not_mem_iff in H.
+        rewrite H. reflexivity.
+      - intros s x H. simpl.
+        case_eq (VSet.mem x s); [|reflexivity].
+        intro HH. f_equal. apply List.map_ext.
+        intros [n y].
+        assert (H': VSet.cardinal (VSet.remove x s) = fuel);
+          [|rewrite H'; reflexivity].
+        apply VSet.mem_spec, VSetProp.remove_cardinal_1 in HH.
+        lia.
+    Qed.
+
+    (* From Equations Require Import Equations. *)
+
+    (* Equations lsp0 (s : VSet.t) (x z : V.t) : Nbar.t by wf (VSet.cardinal s) *)
+    (*   := *)
+    (*   lsp0 s x z := *)
+    (*   let base := if V.eq_dec x z then Some 0 else None in *)
+    (*   match VSet.mem x s as X return VSet.mem x s = X -> _ with *)
+    (*   | true => fun XX => *)
+    (*     let ds := List.map (fun '(n, y) => Some n + lsp0 (VSet.remove x s) y z)%nbar *)
+    (*                        (succs x) in *)
+    (*     List.fold_left Nbar.max ds base *)
+    (*   | false => fun _ => base end eq_refl. *)
+    (* Next Obligation. *)
+    (*   apply VSet.mem_spec in XX. *)
+    (*   pose proof (VSetProp.remove_cardinal_1 XX). *)
+    (*   lia. *)
+    (* Defined. *)
 
     Definition lsp := lsp0 (V G).
 
-    Arguments Nbar.le _ _ : simpl nomatch.
 
     Lemma lsp0_VSet_Equal {s s' x y} :
       VSet.Equal s s' -> lsp0 s x y = lsp0 s' x y.
     Admitted.
+
+    (* Lemma lsp0_VSet_Subset {s s' x y} : *)
+    (*   VSet.Subset s s' -> (lsp0 s x y <= lsp0 s' x y)%nbar. *)
+    (* Admitted. *)
 
     Lemma InAeq_In {A} (l : list A) x :
       InA eq x l <-> In x l.
@@ -604,7 +837,7 @@ Module WeightedGraph (V : UsualOrderedType).
       etransitivity. eapply InA_alt. firstorder. now subst.
     Defined.
     
-    Lemma lsp0_le {s x y} (p : SimplePaths s x y)
+    Lemma lsp0_spec_le {s x y} (p : SimplePaths s x y)
       : (Some (sweight p) <= lsp0 s x y)%nbar.
     Proof.
       induction p; rewrite lsp0_eq; simpl.
@@ -644,7 +877,7 @@ Module WeightedGraph (V : UsualOrderedType).
           cbn. destruct (V.eq_dec x x); [reflexivity|contradiction].
     Qed.
 
-    Lemma lsp0_eq' {s x y} n
+    Lemma lsp0_spec_eq {s x y} n
       : lsp0 s x y = Some n -> exists p : SimplePaths s x y, sweight p = n.
     Proof.
       set (c := VSet.cardinal s). assert (e: VSet.cardinal s = c) by reflexivity.
@@ -686,57 +919,228 @@ Module WeightedGraph (V : UsualOrderedType).
     Qed.
 
 
-
-
-    Definition acyclic_well_founded := well_founded PosPaths.
-    (* Definition acyclic_no_loop := VSet.For_all (fun x => ~ R1s x x) (V G). *)
-    Definition acyclic_no_loop := forall x, ~ (PosPaths x x).
-
-    Lemma acyclic_wf_no_loop : acyclic_well_founded -> acyclic_no_loop.
-    Proof.
-      intros H x. induction (H x).
-      intros [p Hp].
-      destruct p; cbn in Hp. lia.
-      
-    (*   + eapply H1. exact H2. now constructor. *)
-    (*   + eapply H1. exact H2. *)
-    (*     etransitivity. constructor; eassumption. *)
-    (*     now apply clos_tn1_trans. *)
-    (* Qed. *)
-    Abort.
-
     Definition correct_labelling (l : labelling) :=
       l (s G) = 0 /\
       forall e, EdgeSet.In e (E G) -> l e..s + e..w <= l e..t.
 
-    Lemma correct_labelling_R0 l (Hl : correct_labelling l)
-      : forall x y, R0 x y -> l x <= l y.
+    Lemma correct_labelling_Paths l (Hl : correct_labelling l)
+      : forall x y (p : Paths x y), l x + weight p <= l y.
     Proof.
-      intros x y He. apply proj2 in Hl.
-      specialize (Hl _ He); cbn in Hl. lia.
+      induction p. cbn; lia.
+      apply proj2 in Hl.
+      specialize (Hl (x, e..1, y) e..2). cbn in *; lia.
     Qed.
 
-    Lemma correct_labelling_R0s l (Hl : correct_labelling l)
-      : forall x y, R0s x y -> l x <= l y.
+    Lemma acyclic_labelling l : correct_labelling l -> acyclic_no_loop.
     Proof.
-      induction 1. now apply correct_labelling_R0.
-      all: lia.
+      intros Hl x p.
+      specialize (correct_labelling_Paths l Hl x x p); lia.
     Qed.
 
-    Lemma correct_labelling_R l (Hl : correct_labelling l)
-      : forall x y, R1 x y -> l x < l y.
+    Lemma lsp0_triangle_inequality (HG : acyclic_no_loop) s x y1 y2 n
+          (He : EdgeSet.In (y1, n, y2) (E G))
+          (Hy : VSet.In y1 s)
+      : (lsp0 s x y1 + Some n <= lsp0 s x y2)%nbar.
     Proof.
-      intros x y [x' [y' [n [He1 [He2 He3]]]]].
-      apply (correct_labelling_R0s l Hl) in He1.
-      apply (correct_labelling_R0s l Hl) in He3.
-      apply proj2 in Hl. specialize (Hl _ He2); cbn in Hl. lia.
+      case_eq (lsp0 s x y1); [|cbn; trivial].
+      intros m Hm. 
+      apply lsp0_spec_eq in Hm.
+      destruct Hm as [p Hp].
+      case_eq (split p).
+      intros p1 p2 Hp12.
+      pose proof (weight_split p) as H.
+      rewrite Hp12 in H; cbn in H.
+      etransitivity.
+      2: unshelve eapply (lsp0_spec_le (add_end p1 (n; He) _)).
+      subst; rewrite weight_add_end; cbn.
+      pose proof (sweight_weight p2) as HH.
+      rewrite HG in HH. lia.
+      now apply DisjointAdd_remove1.
     Qed.
 
-    Lemma acyclic_labelling l : correct_labelling l -> acyclic_well_founded.
+    Lemma lsp0_xx (HG : acyclic_no_loop) s x
+      : lsp0 s x x = Some 0.
     Proof.
-      intro Hl. eapply Wf_nat.well_founded_lt_compat.
-      exact (correct_labelling_R _ Hl).
+      pose proof (lsp0_spec_le (spaths_refl s x)) as H; cbn in H.
+      case_eq (lsp0 s x x); [|intro e; rewrite e in H; cbn in H; lia].
+      intros n Hn. apply lsp0_spec_eq in Hn.
+      destruct Hn as [p Hp]. rewrite sweight_weight, HG in Hp.
+      subst; reflexivity.
     Qed.
+
+    Definition lsp0_sub {s s' x y}
+      : VSet.Subset s s' -> (lsp0 s x y <= lsp0 s' x y)%nbar.
+    Proof.
+      case_eq (lsp0 s x y); [|cbn; trivial].
+      intros n Hn Hs.
+      apply lsp0_spec_eq in Hn; destruct Hn as [p Hp]; subst.
+      rewrite <- (weight_SimplePaths_sub Hs p).
+      apply lsp0_spec_le.
+    Qed.
+
+    Definition simplify2 {x z} (p : Paths x z)
+      :  forall y (Hy: {VSet.In y (nodes p)} + {x = y}), SimplePaths (nodes p) y z.
+    Proof.
+      induction p.
+      - cbn. intros y [H|H]. 
+        now apply VSetFact.empty_iff in H.
+        subst; reflexivity.
+      - cbn; intros u H.
+        case_eq (VSet.mem u (nodes p)); intro HH.
+        + apply VSet.mem_spec in HH. eapply SimplePaths_sub, IHp.
+          apply VSetProp.subset_add_2; reflexivity. intuition.
+        + assert (X: u = x). {
+            destruct H as [H|H]; [|intuition].
+            apply VSet.add_spec in H; destruct H as [H|H].
+            assumption. apply VSet.mem_spec in H.
+            rewrite H in HH; discriminate. }
+          subst. econstructor. 2: eassumption.
+          2: eapply IHp; now right.
+          split. apply VSetProp.Add_add.
+          now apply VSetFact.not_mem_iff.
+    Defined.      
+
+
+    Lemma nodes_subset {x y} (p : Paths x y)
+      : VSet.Subset (nodes p) (V G).
+    Proof.
+      induction p; cbn.
+      apply VSetProp.subset_empty.
+      apply VSetProp.subset_add_3; [|assumption].
+      apply proj1 in HI.
+      specialize (HI _ e..2); cbn in HI; apply HI.
+    Qed.
+
+    Lemma lsp_s (HG : acyclic_no_loop) x (Hx : VSet.In x (V G))
+      : exists n, lsp (s G) x = Some n.
+    Proof.
+      case_eq (lsp (s G) x).
+      - intros n H; eexists; reflexivity.
+      - intro e.
+        destruct (proj2 (proj2 HI) x Hx) as [p].
+        pose proof (simplify2 p _ (right eq_refl)) as p'.
+        assert (X: (Some (sweight p') <= lsp (s G) x)%nbar). {
+          etransitivity. eapply (lsp0_spec_le p').
+          now eapply lsp0_sub, nodes_subset. }
+        rewrite e in X. inversion X.
+    Qed.
+
+
+    Lemma lsp_correctness (HG : acyclic_no_loop) :
+        correct_labelling (fun x => option_get 0 (lsp (s G) x)).
+    Proof.
+      split.
+      - unfold lsp. now rewrite lsp0_xx.
+      - intros [[x n] y] He; cbn. unfold lsp.
+        simple refine (let H := lsp0_triangle_inequality
+                                  HG (V G) (s G) x y n He _
+                       in _); [|clearbody H].
+        apply proj1 in HI. specialize (HI _ He); cbn in HI; intuition.
+        destruct (lsp_s HG x) as [m Hm].
+        + apply proj1 in HI. apply (HI _ He).
+        + unfold lsp in Hm; rewrite Hm in *; cbn in *.
+        destruct (lsp0 (V G) (s G) y); cbn in *; intuition.
+    Qed.
+
+    Lemma SimplePaths_In {s x y} (p : SimplePaths s x y)
+      : sweight p > 0 -> VSet.In x s.
+    Proof.
+      destruct p. inversion 1.
+      intros _. apply d. left; reflexivity.
+    Qed.
+
+    Lemma acyclic_lsp_xx
+      : acyclic_no_loop <-> (VSet.For_all (fun x => lsp x x = Some 0) (V G)).
+    Proof.
+      split.
+      - intros HG x Hx. now apply lsp0_xx.
+      - intros H. apply acyclic_no_loop_loop'. intros x [p Hp].
+        simple refine (let Hq := weight_simplify p (spaths_refl (V G) _)
+                                                 _ (or_introl Hp)
+                       in _).
+        + exact (V G).
+        + etransitivity. apply VSetProp.union_sym.
+          etransitivity. apply VSetProp.union_subset_equal.
+          apply nodes_subset. reflexivity.
+        + match goal with
+          | _ : 0 < sweight ?qq..2 |- _ => set (q := qq) in *; clearbody Hq
+          end.
+          destruct q as [x' q]; cbn in Hq.
+          assert (Some (sweight q) <= Some 0)%nbar. {
+            erewrite <- H. eapply lsp0_spec_le.
+            eapply SimplePaths_In; eassumption. }
+          cbn in H0; lia.
+    Defined.
+
+
+    (** ** Main results about acyclicity *)
+
+    Lemma acyclic_caract1
+      : acyclic_no_loop <-> exists l, correct_labelling l.
+    Proof.
+      split.
+      intro HG; eexists. eapply (lsp_correctness HG).
+      intros [l Hl]; eapply acyclic_labelling; eassumption.
+    Defined.
+
+    (* Lemma acyclic_caract2 *)
+    (*   : acyclic_no_loop <-> acyclic_well_founded. *)
+    (* Proof. *)
+    (*   split. *)
+    (*   intro. eapply acyclic_labelling. *)
+    (*   now eapply lsp_correctness. *)
+    (*   apply acyclic_wf_no_loop. *)
+    (* Defined. *)
+
+    Lemma acyclic_caract3 :
+      acyclic_no_loop <-> (VSet.For_all (fun x => lsp x x = Some 0) (V G)).
+    Proof.
+      split.
+      - intros HG x Hx. apply lsp0_xx; assumption.
+      - intros H x Hx p.
+    (*     apply R1s_Paths in p. *)
+    (*     destruct p as [p' Hp']. *)
+    (*     pose proof (lsp0_ge_weight _ _ _ p'). rewrite H in H0. *)
+    (*     cbn in *; lia. assumption. *)
+    (* Qed. *)
+    Admitted.
+
+
+    Lemma VSet_Forall_reflect P f (Hf : forall x, reflect (P x) (f x)) s
+      : reflect (VSet.For_all P s) (VSet.for_all f s).
+    Proof.
+      apply iff_reflect. etransitivity.
+      2: apply VSetFact.for_all_iff.
+      2: intros x y []; reflexivity.
+      apply iff_forall; intro x.
+      apply iff_forall; intro Hx.
+      now apply reflect_iff.
+    Qed.
+
+    Lemma reflect_logically_equiv {A B} (H : A <-> B) f
+      : reflect B f -> reflect A f.
+    Proof.
+      destruct 1; constructor; intuition.
+    Qed.
+
+    Definition is_acyclic := VSet.for_all (fun x => match lsp x x with
+                                                 | Some 0 => true
+                                                 | _ => false
+                                                 end) (V G).
+
+    Lemma is_acyclic_correct : reflect acyclic_no_loop is_acyclic.
+    Proof.
+      eapply reflect_logically_equiv. eapply acyclic_caract3.
+      apply VSet_Forall_reflect; intro x.
+      destruct (lsp x x). destruct n. constructor; reflexivity.
+      all: constructor; discriminate.
+    Qed.
+
+
+
+
+
+
 
     Definition get_edges x y :=
       let L := List.filter
@@ -760,6 +1164,21 @@ Module WeightedGraph (V : UsualOrderedType).
       cbn. destruct (V.eq_dec x' x); destruct (V.eq_dec y' y); intuition; subst.
       reflexivity. all: inversion H0; intuition.
     Qed.
+
+    Definition acyclic_well_founded := well_founded PosPaths.
+
+    Lemma acyclic_wf_no_loop : acyclic_well_founded -> acyclic_no_loop.
+    Proof.
+      intros H x. induction (H x).
+      intros [p Hp].
+      destruct p; cbn in Hp. lia.
+      
+    (*   + eapply H1. exact H2. now constructor. *)
+    (*   + eapply H1. exact H2. *)
+    (*     etransitivity. constructor; eassumption. *)
+    (*     now apply clos_tn1_trans. *)
+    (* Qed. *)
+    Abort.
 
 
     Import Nbar.
@@ -1154,37 +1573,6 @@ Module WeightedGraph (V : UsualOrderedType).
       intuition.
     Qed.
 
-    Lemma lsp_correctness (HG : acyclic_no_loop) :
-        correct_labelling (fun x => option_get 0 (lsp (s G) x)).
-    Proof.
-      split.
-      - unfold lsp. rewrite lsp0_xx. reflexivity. assumption.
-        apply HI.
-      - intros [[x n] y] He; cbn. unfold lsp.
-        simple refine (let H := lsp0_triangle_inequality
-                                  HG (VSet.elements (V G)) (s G) x y n He _
-                       in _); [|clearbody H].
-        apply proj1 in HI. specialize (HI _ He).
-        apply proj1, InA_alt in HI. destruct HI as [? [[] ?]]; assumption.
-        simple refine (let H1 := Paths_lsp0_finite
-                                   (VSet.elements (V G)) (s G) x _ in _);
-          [|destruct H1 as [n1 H1]].
-        apply Rs_Paths. apply HI.
-        apply proj1 in HI. specialize (HI _ He); apply HI.
-        simple refine (let H2 := Paths_lsp0_finite
-                                   (VSet.elements (V G)) (s G) y _ in _);
-          [|destruct H2 as [n2 H2]].
-        apply Rs_Paths. apply HI.
-        apply proj1 in HI. specialize (HI _ He); apply HI.
-        now rewrite H1, H2 in *.
-    Defined.
-
-    
-    Lemma notR1s_correct_labelling
-      : acyclic_no_loop -> exists l, correct_labelling l.
-    Proof.
-      intro HG; eexists. eapply (lsp_correctness HG).
-    Defined.
 
     (* Lemma weight_morphism x y z p1 p2 *)
     (*   : weight (@Paths_trans x y z p1 p2) = weight p1 + weight p2. *)
@@ -1230,68 +1618,6 @@ Module WeightedGraph (V : UsualOrderedType).
         (* rewrite weight_Paths_trans0 *)
     Abort.
 
-    (** ** Main results about acyclicity *)
-
-    Lemma acyclic_caract1
-      : acyclic_no_loop <-> exists l, correct_labelling l.
-    Proof.
-      split. apply notR1s_correct_labelling.
-      intro. apply acyclic_wf_no_loop.
-      destruct H; eapply acyclic_labelling; eassumption.
-    Defined.
-
-    Lemma acyclic_caract2
-      : acyclic_no_loop <-> acyclic_well_founded.
-    Proof.
-      split.
-      intro. eapply acyclic_labelling.
-      now eapply lsp_correctness.
-      apply acyclic_wf_no_loop.
-    Defined.
-
-    Lemma acyclic_caract3 :
-      acyclic_no_loop <-> (VSet.For_all (fun x => lsp x x = Some 0) (V G)).
-    Proof.
-      split.
-      - intros HG x Hx. apply lsp0_xx; assumption.
-      - intros H x Hx p.
-    (*     apply R1s_Paths in p. *)
-    (*     destruct p as [p' Hp']. *)
-    (*     pose proof (lsp0_ge_weight _ _ _ p'). rewrite H in H0. *)
-    (*     cbn in *; lia. assumption. *)
-    (* Qed. *)
-    Admitted.
-
-
-    Lemma VSet_Forall_reflect P f (Hf : forall x, reflect (P x) (f x)) s
-      : reflect (VSet.For_all P s) (VSet.for_all f s).
-    Proof.
-      apply iff_reflect. etransitivity.
-      2: apply VSetFact.for_all_iff.
-      2: intros x y []; reflexivity.
-      apply iff_forall; intro x.
-      apply iff_forall; intro Hx.
-      now apply reflect_iff.
-    Qed.
-
-    Lemma reflect_logically_equiv {A B} (H : A <-> B) f
-      : reflect B f -> reflect A f.
-    Proof.
-      destruct 1; constructor; intuition.
-    Qed.
-
-    Definition is_acyclic := VSet.for_all (fun x => match lsp x x with
-                                                 | Some 0 => true
-                                                 | _ => false
-                                                 end) (V G).
-
-    Lemma is_acyclic_correct : reflect acyclic_no_loop is_acyclic.
-    Proof.
-      eapply reflect_logically_equiv. eapply acyclic_caract3.
-      apply VSet_Forall_reflect; intro x.
-      destruct (lsp x x). destruct n. constructor; reflexivity.
-      all: constructor; discriminate.
-    Qed.
     
     Definition leq_vertices x y := forall l, correct_labelling l -> l x <= l y.
 
